solve the two interesting [admit]s in [namei_ok]
now just need to prove three lemmas about fold_left: one for extracting
[None] when the name is not there, one for extracting a [DirFile] when
[isdir] is 0, and one for extracting a [DirSubdir] when [isdir] is 1.

src/DirTree.v
@@ -75,37 +75,39 @@ Module DIRTREE.
   Definition tree_pred (dirlist : dirtree) :=
     tree_pred' diritem_pred dirlist.
 
-  Definition rep fsxp tree :=
+  Definition rep fsxp rootinum tree :=
     (exists bflist freeinodes freeinode_pred_unused freeinode_pred,
      BFILE.rep fsxp.(FSXPBlockAlloc) fsxp.(FSXPInode) bflist *
      BALLOC.rep_gen fsxp.(FSXPInodeAlloc) freeinodes freeinode_pred_unused freeinode_pred *
-     [[ (tree_dir_names_pred fsxp.(FSXPRootInum) tree * tree_pred tree * freeinode_pred)%pred (list2nmem bflist) ]]
+     [[ (tree_dir_names_pred rootinum tree * tree_pred tree * freeinode_pred)%pred (list2nmem bflist) ]]
     )%pred.
 
-  Lemma tree_dir_extract : forall d F dmap name inum,
-    (F * name |-> (inum, $1))%pred dmap
+  Lemma tree_dir_extract : forall d F dmap name inum isdir,
+    (F * name |-> (inum, isdir))%pred dmap
+    -> isdir <> $0
     -> tree_dir_names_pred' d dmap
     -> tree_pred d =p=> exists F s, F * tree_dir_names_pred inum s * tree_pred s.
   Proof.
     induction d; intros.
-    - simpl in *. eapply emp_complete in H0; [| apply emp_empty_mem ]; subst.
+    - simpl in *. eapply emp_complete in H1; [| apply emp_empty_mem ]; subst.
       apply sep_star_empty_mem in H; intuition.
       exfalso. eapply ptsto_empty_mem. eauto.
     - destruct a. destruct p. destruct d0; simpl in *.
-      + apply ptsto_mem_except in H0 as H0'.
+      + apply ptsto_mem_except in H1 as H1'.
         rewrite IHd. cancel. cancel.
-        2: eauto.
+        2: eauto. 2: eauto.
         apply sep_star_comm in H.
-        pose proof (ptsto_diff_ne H0 H).
-        destruct (string_dec name s). exfalso. apply H1; eauto. discriminate.
+        pose proof (ptsto_diff_ne H1 H).
+        destruct (string_dec name s). exfalso. apply H2; eauto.
+        destruct (weq isdir $0); try congruence.
         apply sep_star_comm. eapply ptsto_mem_except_exF; eauto.
       + destruct (string_dec name s); subst.
-        * apply ptsto_valid in H0. apply ptsto_valid' in H.
-          rewrite H in H0. inversion H0. subst.
+        * apply ptsto_valid in H1. apply ptsto_valid' in H.
+          rewrite H in H1. inversion H1. subst.
           cancel. unfold tree_pred. instantiate (a0:=l). cancel.
-        * apply ptsto_mem_except in H0.
+        * apply ptsto_mem_except in H1.
           rewrite IHd. cancel. cancel.
-          2: eauto.
+          2: eauto. 2: eauto.
           apply sep_star_comm. eapply ptsto_mem_except_exF; eauto.
           pred_apply; cancel.
   Qed.
@@ -118,8 +120,9 @@ Module DIRTREE.
       Invariant
         MEMLOG.rep fsxp.(FSXPMemLog) (ActiveTxn mbase m) mscs_inum_isdir.(fst).(fst) *
         exists tree,
-        [[ (F * rep fsxp treetop)%pred (list2mem m) ]] *
-        [[ (exists F', tree_dir_names_pred mscs_inum_isdir.(fst).(snd) tree *
+        [[ (F * rep fsxp dnum treetop)%pred (list2mem m) ]] *
+        [[ mscs_inum_isdir.(snd) <> $0 ->
+           (exists F', tree_dir_names_pred mscs_inum_isdir.(fst).(snd) tree *
             tree_pred tree * F')%pred (list2nmem bflist) ]] *
         [[ find_name treetop fnlist dnum $1 = find_name tree fn mscs_inum_isdir.(fst).(snd) mscs_inum_isdir.(snd) ]]
       OnCrash
@@ -141,7 +144,7 @@ Module DIRTREE.
   Theorem namei_ok : forall fsxp dnum fnlist mscs,
     {< F mbase m tree,
     PRE    MEMLOG.rep fsxp.(FSXPMemLog) (ActiveTxn mbase m) mscs *
-           [[ (F * rep fsxp tree)%pred (list2mem m) ]]
+           [[ (F * rep fsxp dnum tree)%pred (list2mem m) ]]
     POST:(mscs,r)
            [[ r = find_name tree fnlist dnum $1 ]] *
            MEMLOG.rep fsxp.(FSXPMemLog) (ActiveTxn mbase m) mscs
@@ -153,60 +156,55 @@ Module DIRTREE.
 
     instantiate (a4 := l).
     pred_apply. cancel.
-    (*
-     * interesting problem: [namei] starts from a caller-supplied directory, but
-     * we don't have a precondition proving that this directory [dnum] is a valid
-     * part of the tree..
-     *)
-    admit.
 
     step.
     step.
     destruct (weq b $0); congruence.
 
     (* destruct some [exists] terms before creating evars.. *)
-    unfold tree_dir_names_pred in H11; destruct_lift H11.
+    eapply pimpl_ok2; [ eauto with prog |].
+    intros; norm'l; unfold stars; simpl.
+    apply H11 in H14 as H14'.
+    unfold tree_dir_names_pred in H14'; destruct_lift H14'.
 
-    step.
+    cancel.
     unfold SDIR.rep_macro. do 2 eexists. intuition.
-    (* Be careful which [list2mem d0] we pick! *)
+    (* Be careful which [list2mem] we pick! *)
     eapply pimpl_apply; [ | exact H3 ]. cancel.
-    pred_apply. cancel.
+    eapply pimpl_apply; [ | exact H0 ]. cancel.
     eauto.
 
     destruct b3.
-
     destruct p6.
     eapply pimpl_ok2; eauto.
     intros; norm'l; split_or_l; unfold stars; simpl;
       norm'l; unfold stars; simpl; inv_option_eq.
 
-    (* we probably have an overly strong loop invariant..  we need to know that
-     * for the next loop iteration, [isdir] is $1, since otherwise we don't
-     * have a [tree_dir_names_pred].
-     *)
-    assert (a2 = $1) by admit.
-    subst.
-    rewrite tree_dir_extract in H0 by eauto; destruct_lift H0.
+    rewrite H10; clear H10. destruct (weq b $0); try congruence.
+    (* check whether, for the next loop iteration, [isdir] is $0 or $1 *)
+    destruct (weq a2 $0).
+    cancel.
+
+    (* extract a DirFile from the [fold_left] *)
+    admit.
+
+    rewrite tree_dir_extract in H0 by eauto. destruct_lift H0.
     cancel.
     instantiate (a0 := d3). cancel.
-    destruct (weq b $0); try congruence.
-    rewrite H10.
 
-    (* extract the element out of the [fold_left].. *)
+    (* extract a DirSubdir from the [fold_left] *)
     admit.
 
     step.
-    destruct (weq b $0); try congruence.
-    rewrite H10.
+    rewrite H10; clear H10. destruct (weq b $0); try congruence.
 
-    (* extract a non-existent element [elem] out of the [fold_left] to produce [None].. *)
+    (* extract a non-existent element [elem] out of the [fold_left] to produce [None] *)
     admit.
 
     step.
 
     Grab Existential Variables.
-    exact emp.
+    exact nil.
   Qed.
 
   Definition mknod T fsxp dnum name isdir mscs rx : prog T :=
